commit

AP/AP/Defense/Box.lean
@@ -7,5 +7,20 @@ def offset : ℕ := 106
 def corners : List Corner :=
   Dir.univList.map (⟨·, offset⟩)
 
+def defenses : List Defense :=
+  corners.map (·.defense)
+
 def defense : Defense :=
-  .ofList # corners.map (·.defense)
+  .ofList defenses
+
+-----
+
+theorem compatible_of_mem_defenses {c₁ c₂}
+(h₁ : c₁ ∈ defenses) (h₂ : c₂ ∈ defenses) : c₁.Compatible c₂ := by
+  sorry
+
+-- #check 0 #exit
+
+@[simp]
+instance : defense.WF :=
+  Defense.wf_ofList (by simp [defenses]) compatible_of_mem_defenses
